Setoids

theories/TransitionSystem.v
@@ -1,32 +1,3 @@
-From Coq Require Import
-  Program
-  List
-  Ensembles
-  Relation_Definitions
-  RelationClasses
-  SetoidClass
-  SetoidDec.
-
-Section exists_equiv.
-  Context {S : Type} `{Setoid S}.
-
-  Definition exists_equiv (prop : S -> Prop) (s : S) : Prop :=
-    exists (s' : S), prop s' /\ s == s'.
-End exists_equiv.
-
-Notation "'exists{' A == B } , C" := (exists_equiv (fun A => C) B) (at level 300, A name, B name, C at level 300, right associativity) : type_scope.
-
-Hint Unfold exists_equiv : slot.
-
-Section covariant_relation.
-  Context {State : Type} `{Setoid State} (R : relation State).
-
-  Definition rel_covariant :=
-    forall (s1 s2 s1' : State),
-      s1 == s2 ->
-      R s1 s1' ->
-      exists{s2' == s1'}, R s2 s2'.
-End covariant_relation.
 
 Section defn.
   Context {State Arrow Result : Type}.
@@ -73,15 +44,12 @@ Section props.
   Lemma compose_covariance (a b : relation State) (Hcov_a : rel_covariant a) (Hcov_b : rel_covariant b) :
     rel_covariant (a ∘ b).
   Proof.
-    intros s1 s2 s1'' Heq Hs1''.
-    destruct Hs1'' as [s1' Hs1' Hs1''].
+    intros s1 s2 s1'' Heq [s1' Hs1' Hs1''].
     specialize (Hcov_a s1 s2 s1' Heq Hs1').
     destruct Hcov_a as [s2' [Hs2' Heq']].
     specialize (Hcov_b s1' s2' s1'' Heq' Hs1'').
     destruct Hcov_b as [s2'' [Hs2'' Heq'']].
-    exists s2''. split.
-    - econstructor; eauto.
-    - assumption.
+    exists s2''. sauto.
   Qed.
 
   Definition commutative (a b : relation State) : Prop :=
@@ -94,10 +62,7 @@ Section props.
       ((b ∘ a) s s1' -> exists{s2' == s1'}, (a ∘ b) s s2').
 End props.
 
-From Hammer Require Import
-  Tactics.
-
-Theorem eq_setoid_commutative `{HST : StrictTransitionSystem} :
+Fact eq_setoid_commutative `{HST : StrictTransitionSystem} :
   forall a b,
     commutative a b <-> @setoid_commutative _ _ _ HST leibnizTS a b.
 Proof.
@@ -121,27 +86,60 @@ Section trace.
       Trace trace s' s'' ->
       Trace (arrow :: trace) s s''.
 
-  Fixpoint trace_via_compose (t : list Arrow) : relation State :=
+  Fixpoint trace_via_compose (t : list (relation State)) : relation State :=
     match t with
     | [] => eq
-    | (a :: t) => (ts_morph a) ∘ trace_via_compose t
+    | [a] => a
+    | (a :: t) => a ∘ trace_via_compose t
     end.
 
-  Lemma trace_is_compose_fold :
+  Fact trace_is_compose_fold :
     forall t s s',
-      Trace t s s' <-> trace_via_compose t s s'.
-  Proof with easy.
+      Trace t s s' <-> trace_via_compose (map ts_morph t) s s'.
+  Proof with sauto.
     intros t s s''.
     split.
     - intros Ht. induction Ht.
       + easy.
-      + simpl. unfold compose.
-        exists s'...
+      + simpl in *.
+        destruct trace.
+        * sauto.
+        * simpl.
+          exists s'.
+          -- assumption.
+          -- apply IHHt.
     - generalize dependent s. induction t; intros s Ht; simpl in Ht.
       + rewrite Ht. constructor.
-      + destruct Ht as [s' Hs' Hs''].
-        specialize (IHt s' Hs'').
-        constructor 2 with (s' := s')...
+      + destruct t; simpl in Ht.
+        * constructor 2 with (s' := s'')...
+        * inversion Ht.
+          specialize (IHt x).
+          constructor 2 with (s' := x); [assumption|].
+          simpl in IHt. apply IHt in H1.
+          assumption.
+  Qed.
+
+  Lemma trace_split : forall s s'' t1 t2,
+      Trace (t1 ++ t2) s s''  ->
+      exists s', Trace t1 s s' /\ Trace t2 s' s''.
+  Proof with sauto.
+    intros.
+    generalize dependent s.
+    induction t1; intros.
+    - exists s...
+    - simpl in H0. inversion H0. subst. clear H0.
+      destruct (IHt1 s' H6) as [s_ [Ht1 Ht2]].
+      exists s_. split; sauto.
+  Qed.
+
+  Lemma trace_concat : forall s s' s'' t1 t2,
+      Trace t1 s s' ->
+      Trace t2 s' s'' ->
+      Trace (t1 ++ t2) s s''.
+  Proof with sauto.
+    intros.
+    generalize dependent s.
+    induction t1...
   Qed.
 
   Lemma trace_equiv_covariance :
@@ -164,7 +162,7 @@ Section trace.
   Qed.
 
   Lemma trace_via_compose_eqiuv_covariance :
-    forall t, rel_covariant (trace_via_compose t).
+    forall t, rel_covariant (trace_via_compose (map ts_morph t)).
   Proof.
     intros t s s1 s2 s1' Ht.
     rewrite <-trace_is_compose_fold in Ht.
@@ -173,3 +171,110 @@ Section trace.
     rewrite <-trace_is_compose_fold. easy.
   Qed.
 End trace.
+
+
+Definition morph_setoid_commutative `{TransitionSystem} a b := setoid_commutative (ts_morph a) (ts_morph b).
+
+Definition can_follow `{TransitionSystem} `{CanonicalOrder Arrow} (a b : Arrow) :=
+  (canon_rel a b = true) \/ (~morph_setoid_commutative a b).
+
+
+Definition TraceEnsemble {Arrow : Type} := Ensemble (list Arrow).
+
+Section trace_equivalence.
+  Context `{T : TransitionSystem} (e e' : @TraceEnsemble Arrow).
+
+  Definition sufficient_replacement :=
+    forall t s s'1, e t ->
+              Trace t s s'1 ->
+              exists t' s'2, e' t' /\ Trace t' s s'2 /\ s'1 == s'2.
+
+  Definition sufficient_replacement_p :=
+    forall t, e t ->
+         exists t', e' t' /\ RestrictedPermutation morph_setoid_commutative t t'.
+
+  Lemma trace_commut_swap2 a b s s'1 :
+    morph_setoid_commutative a b->
+    Trace [a; b] s s'1 ->
+    exists{s'2 == s'1}, Trace [b; a] s s'2.
+  Proof.
+    intros.
+    apply trace_is_compose_fold in H1. simpl in H1.
+    destruct (H0 s s'1) as [Hcomm _].
+    destruct (Hcomm H1) as [s'2 [H2 Hs'2]].
+    exists s'2. split.
+    - now rewrite trace_is_compose_fold.
+    - assumption.
+  Qed.
+
+  Lemma trace_commutative_permutation s s'1 t t' :
+    Trace t s s'1 ->
+    RestrictedPermutation morph_setoid_commutative t t' ->
+    exists{s'2 == s'1}, Trace t' s s'2.
+  Proof with easy.
+    intros Hls Hperm.
+    generalize dependent s. generalize dependent s'1.
+    induction Hperm; intros.
+    - exists s. sauto.
+    - inversion Hls; subst; clear Hls.
+      specialize (IHHperm s'1 s' H5).
+      destruct IHHperm as [s'2 [Hs'2 Hl2]].
+      exists s'2; split.
+      + now constructor 2 with (s' := s').
+      + assumption.
+    - replace (a :: b :: l) with ([a; b] ++ l) in Hls by reflexivity.
+      replace (b :: a :: l) with ([b; a] ++ l) by reflexivity.
+      apply trace_split in Hls. destruct Hls as [s' [Hab Hls]].
+      apply trace_commut_swap2 in Hab; [|assumption].
+      destruct Hab as [s_ [Hsl_ Hs_]].
+      specialize (trace_equiv_covariance l s' s_ s'1 Hs_ Hls) as Hls_.
+      destruct Hls_ as [s'2 [Hls_ Hs'2]].
+      exists s'2. split; [|assumption].
+      apply trace_concat with (s' := s_)...
+    - specialize (IHHperm1 s'1 s Hls).
+      destruct IHHperm1 as [s'2 [Hls'2 Hs'2]].
+      specialize (IHHperm2 s'2 s Hls'2).
+      destruct IHHperm2 as [s'3 [Hls'3 Hs'3]].
+      exists s'3. split.
+      + assumption.
+      + rewrite Hs'2...
+  Qed.
+
+  (* Lemma comm_perm_sufficient_replacement : *)
+  (*   sufficient_replacement_p -> *)
+  (*   sufficient_replacement. *)
+  (* Proof. *)
+  (*   intros Hsrp t s s'1 Het Hs'1. *)
+  (*   specialize (Hsrp t Het). clear Het. *)
+  (*   destruct Hsrp as [t' [He't' Hperm]]. *)
+  (*   generalize dependent s. generalize dependent s'1. *)
+  (*   induction Hperm; intros s s'1 Ht. *)
+  (*   - sauto. *)
+  (*   -  *)
+
+
+
+
+    -
+    induction Hperm.
+    - intros s s'1 He_t Hs'1.
+      exists []. exists s.
+      inversion Hs'1; subst.
+      repeat split.
+      +
+
+    intros Hsrp t s s' Ht Hls.
+    destruct (Hsrp t Ht) as [t' [Ht' Hperm]].
+    induction Hperm.
+    - exists []. exists s. repeat split.
+      + assumption.
+      + constructor.
+      + inversion Hls. apply reflexivity.
+    - inversion Hls; subst; clear Hls.
+      assert (e l1). {
+
+      specialize (IHHperm
+
+    eapply trace_commutateive_permutation in Hperm; eauto.
+  Qed.
+End trace_equivalence.
