theories/Multifunction.v
@@ -1,0 +1,693 @@
+From Coq Require Import
+  Program
+  Decidable
+  List
+  Ensembles
+  Relation_Definitions
+  RelationClasses
+  SetoidClass
+  SetoidDec
+  Classes.Morphisms.
+
+From Hammer Require Import
+  Tactics.
+
+From SLOT Require Import
+  RestrictedPermutation.
+
+Import ListNotations.
+
+Section exists_equiv.
+  Context {S : Type} `{Setoid S}.
+
+  Definition exists_equiv (prop : S -> Prop) (s : S) : Prop :=
+    exists (s' : S), prop s' /\ s == s'.
+End exists_equiv.
+
+Notation "'exists{' A == B } , C" :=
+  (exists_equiv (fun A => C) B)
+  (at level 300, A name, B name, C at level 300, right associativity) : type_scope.
+
+Hint Unfold exists_equiv : slot.
+
+Section mfun.
+  Context (A B : Type) `{Setoid A} `{Setoid B}.
+
+  Structure MFun : Type := {
+      morphism : A -> B -> Prop;
+      morphism_covariance : forall x x' y,
+        x == x' ->
+        morphism x y ->
+        exists{y' == y}, morphism x' y';
+    }.
+End mfun.
+
+Global Arguments morphism {_ _ _ _}.
+Global Arguments morphism_covariance {_ _ _ _}.
+
+Notation "A '~[' B ']~>' C" := (morphism B A C) (at level 20) : slot_scope.
+Open Scope slot_scope.
+
+Ltac morph_shift morphism point :=
+  lazymatch goal with
+  | [Hequiv : point == ?A, Hmorph : ?A ~[morphism]~> ?B |- _] =>
+      symmetry in Hequiv; morph_shift point morphism
+  | [Hequiv : ?A == point, Hmorph : ?A ~[morphism]~> ?B |- _] =>
+      let B' := fresh B "'" in
+      let Hequiv' := fresh "Hequiv_" B "_" B' in
+      let Hmorph' := fresh "Hmorph_" point "_" B' in
+      idtac "equiv=" Hequiv "morph=" Hmorph "B'=" B';
+      destruct (morphism_covariance _ _ _ _ Hequiv Hmorph) as [B' [Hmorph' Hequiv']]
+  end.
+
+Section compose.
+  Context {A B C : Type} `{HA : Setoid A} `{HB : Setoid B} `{HC : Setoid C}.
+
+  Let F := @MFun A B HA HB.
+  Let G := @MFun B C HB HC.
+
+  Program Definition compose (f : F) (g : G) : MFun A C :=
+     {| morphism := fun x z => exists y, morphism f x y /\ morphism g y z; |}.
+  Next Obligation.
+    rename y into z. rename H0 into y.
+    morph_shift f x'.
+    morph_shift g y'.
+    exists z'. sauto.
+  Qed.
+End compose.
+
+Infix "∘" := compose : slot_scope.
+
+Section props.
+  Context {A : Type} `{Hsetoid : Setoid A}.
+  Let T := @MFun A A Hsetoid Hsetoid.
+
+  Definition eq_commute (f g : T) :=
+    forall (x y : A), x ~[f ∘ g]~> y <-> x ~[g ∘ f]~> y.
+
+  Definition commute (f g : T) :=
+    forall x y,
+      (x ~[f ∘ g]~> y -> exists{y' == y}, x ~[g ∘ f]~> y') /\
+      (x ~[g ∘ f]~> y -> exists{y' == y}, x ~[f ∘ g]~> y').
+
+  Program Definition id_mfun : T :=
+    {| morphism := eq; |}.
+  Next Obligation.
+    exists x'; easy.
+  Qed.
+
+  Fixpoint compose_list (l : list T) : T :=
+    match l with
+    | [] => id_mfun
+    | [a] => a
+    | (a :: l) => a ∘ compose_list l
+    end.
+
+  Lemma compose_list_split (l1 l2 : list T) x z :
+    x ~[compose_list (l1 ++ l2)]~> z ->
+    exists y,
+      x ~[compose_list l1]~> y /\
+      y ~[compose_list l2]~> z.
+  Proof.
+    generalize dependent x.
+    induction l1; intros x H.
+    - simpl in H.
+      exists x. split; easy.
+    - simpl in H.
+      remember (l1 ++ l2) as l.
+      destruct l.
+      + symmetry in Heql. destruct (app_eq_nil _ _ Heql) as [Hl1 Hl2].
+        subst. exists z. firstorder.
+      + destruct H as [w [Hxw Hwz]].
+        rewrite Heql in *.
+        destruct (IHl1 _ Hwz) as [mid [Hwmid Hmidz]].
+        exists mid. split.
+        2:{ assumption. }
+        destruct l1.
+        * simpl in *. subst. assumption.
+        * simpl. exists w; firstorder.
+  Qed.
+
+  Lemma compose_list_app (l1 l2 : list T) x y z :
+    x ~[compose_list l1]~> y ->
+    y ~[compose_list l2]~> z ->
+    x ~[compose_list (l1 ++ l2)]~> z.
+  Proof.
+    generalize dependent x. generalize dependent y.
+    induction l1; intros x y Hl1 Hl2.
+    - simpl in *. subst. assumption.
+    - destruct l1.
+      + simpl in Hl1.
+        destruct l2 as [|g l2].
+        * simpl in *. now subst.
+        * exists x.
+          rewrite app_nil_l.
+          firstorder.
+      + destruct Hl1 as [w [Hyw Hwx]].
+        specialize (IHl1 x w Hwx Hl2).
+        exists w. firstorder.
+  Qed.
+
+  Lemma comm_permutation (l l' : list T) x y :
+    RestrictedPermutation commute l l' ->
+    x ~[compose_list l]~> y ->
+    exists{y' == y}, x ~[compose_list l']~> y'.
+  Proof.
+    intros Hperm. generalize dependent x. generalize dependent y.
+    induction Hperm as [| f l1 l2 | |]; intros y x.
+    { simpl. exists y. subst. split; reflexivity. }
+    { intros Hfl1.
+      replace (f :: l1) with ([f] ++ l1) in Hfl1 by reflexivity.
+      apply compose_list_split in Hfl1. destruct Hfl1 as [w [Hxw Hwy]].
+      specialize (IHHperm y w Hwy). destruct IHHperm as [z [Hwz Hz]].
+      exists z. split.
+      - replace (f :: l2) with ([f] ++ l2) by reflexivity.
+        eapply compose_list_app; now eauto.
+      - assumption.
+    }
+    { replace (a :: b :: l) with ([a; b] ++ l) by reflexivity.
+      replace (b :: a :: l) with ([b; a] ++ l) by reflexivity.
+      intros Hxy.
+      apply compose_list_split in Hxy. destruct Hxy as [w [Hxw Hwy]].
+      destruct (H x w) as [Hcomm _].
+      destruct Hcomm as [v [Hxv Hv]].
+      - inversion Hxw. firstorder.
+      - morph_shift (compose_list l) v.
+        exists y'.
+        split.
+        + eapply compose_list_app; eauto.
+        + assumption.
+    }
+    { intros Hl.
+      eapply IHHperm1 in Hl. destruct Hl as [y1 [Hxy1 Hyy1]].
+      eapply IHHperm2 in Hxy1. destruct Hxy1 as [y2 [Hy2 Hy1y2]].
+      exists y2. split.
+      - assumption.
+      - rewrite Hyy1, Hy1y2. reflexivity.
+    }
+  Qed.
+End props.
+
+Fact eq_setoid_commutative {A} (a b : @MFun A A (eq_setoid A) (eq_setoid A)) :
+  eq_commute a b <-> commute a b.
+Proof.
+  split; unfold commute, eq_commute.
+  - sauto.
+  - intros H x z. specialize (H x z).
+    sauto.
+Qed.
+
+Section setoid_pair.
+  Context (A B : Type) `{Setoid A} `{Setoid B}.
+
+  Program Instance setoidPair : Setoid (A * B) :=
+    {| equiv (a b : (A * B)) :=
+        let (a_l, a_r) := a in
+        let (b_l, b_r) := b in
+        equiv a_l b_l /\ equiv a_r b_r;
+    |}.
+  Next Obligation.
+    sauto unfold:Reflexive,Symmetric,Transitive.
+  Qed.
+End setoid_pair.
+
+Section mfun_prod.
+  Context {A B C D : Type} `{setoidA : Setoid A} `{setoidB : Setoid B} `{setoidC : Setoid C} `{setoidD : Setoid D}.
+
+  Program Definition mfun_prod (f : @MFun A B setoidA setoidB) (g : @MFun C D setoidC setoidD) :
+    @MFun (A * C) (B * D) (setoidPair A C) (setoidPair B D) :=
+    {| morphism x y :=
+        let (x_l, x_r) := x in
+        let (y_l, y_r) := y in
+        morphism f x_l y_l /\ morphism g x_r y_r;
+    |}.
+  Next Obligation.
+    morph_shift f a.
+    morph_shift g c.
+    exists (b', d'). sauto.
+  Qed.
+End mfun_prod.
+
+Section mfun_sum.
+  Context {A A' B : Type} `{setoidA : Setoid A} `{setoidA' : Setoid A'} `{setoidB : Setoid B}.
+
+  Program Definition mfun_sum_l (f : @MFun A A' setoidA setoidA') :
+    @MFun (A * B) (A' * B) (setoidPair A B) (setoidPair A' B) :=
+    {| morphism x y :=
+        let (x_l, x_r) := x in
+        let (y_l, y_r) := y in
+        morphism f x_l y_l /\ x_r = y_r
+    |}.
+  Next Obligation.
+    morph_shift f a0.
+    exists (a', b0).
+    sauto.
+  Qed.
+
+  Program Definition mfun_sum_r (f : @MFun A A' setoidA setoidA') :
+    @MFun (B * A) (B * A') (setoidPair B A) (setoidPair B A') :=
+    {| morphism x y :=
+        let (x_l, x_r) := x in
+        let (y_l, y_r) := y in
+        x_l = y_l /\ morphism f x_r y_r
+    |}.
+  Next Obligation.
+    morph_shift f a0.
+    exists (b0, a').
+    sauto.
+  Qed.
+End mfun_sum.
+
+Section ensembles.
+  Context (A : Type) `{Hsetoid : Setoid A}.
+  Let M := @MFun A A Hsetoid Hsetoid.
+
+  Definition TraceEnsemble := Ensemble (list M).
+
+  Definition sufficient_replacement_p e e' :=
+    forall t, e t ->
+              exists t', e' t' /\ RestrictedPermutation commute t t'.
+End ensembles.
+
+Section canonical_order.
+  Context {A : Type}.
+
+  Class CanonicalOrder (canon_rel : relation A) := {
+      canon_rel_dec a b : decidable (canon_rel a b);
+
+      canon_total a b : canon_rel a b \/ canon_rel b a;
+
+      canon_trans :: Transitive canon_rel;
+      (* Reflexivity is important for ordering of events produced by
+      the same process: *)
+      canon_reflexive :: Reflexive canon_rel;
+      canon_antisymmetric a b := canon_rel a b -> canon_rel b a -> a = b;
+    }.
+End canonical_order.
+
+Section canonical_trace.
+  Context {A : Type} `{Hsetoid : Setoid A}.
+  Let M := @MFun A A Hsetoid Hsetoid.
+  Context `{Hcanon : CanonicalOrder M}.
+  Context (commut_dec : forall f g, decidable (commute f g)).
+
+  Definition can_follow (a b : M) :=
+    (~commute a b) \/ (canon_rel a b).
+
+  Lemma can_follow_dec a b : decidable (can_follow a b).
+  Proof.
+    unfold can_follow.
+    specialize (commut_dec a b) as Hdcomm.
+    apply dec_not in Hdcomm.
+    apply dec_or.
+    + assumption.
+    + apply canon_rel_dec.
+  Qed.
+
+  Definition can_follow_hd (label : M) (trace : list M) : Prop :=
+    match trace with
+    | [] => True
+    | head :: _ =>
+        can_follow label head
+    end.
+
+  Lemma can_follow_hd_dec a t : decidable (can_follow_hd a t).
+  Proof.
+    destruct t.
+    - simpl. apply dec_True.
+    - simpl. apply can_follow_dec.
+  Qed.
+
+  Inductive CanonicalTrace : list M -> relation A :=
+  | canontr_nil : forall s,
+      CanonicalTrace [] s s
+  | canontr_cons : forall s s' s'' label trace,
+      s ~[label]~> s' ->
+      can_follow_hd label trace ->
+      CanonicalTrace trace s' s'' ->
+      CanonicalTrace (label :: trace) s s''.
+
+  Program Definition mfunCanonTrace t := {| morphism := CanonicalTrace t |}.
+  Next Obligation.
+    generalize dependent x'.
+    induction H0 as [|x y z f t Hfxy Hfollow Ht IH].
+    - sauto.
+    - intros a2 Hx.
+      morph_shift f a2.
+      destruct (IH y' Hequiv_y_y') as [z' [Hy'z' Hzz']].
+      exists z'. split.
+      + constructor 2 with (s' := y'); sauto.
+      + assumption.
+  Qed.
+
+  Lemma can_follow_hd_eq {te t1 t2} (Hfoll : can_follow_hd te t1) (Hhd : hd_error t1 = hd_error t2) :
+    can_follow_hd te t2.
+  Proof.
+    intros.
+    unfold can_follow_hd in *.
+    destruct t1, t2; try reflexivity.
+    - exfalso. inversion Hhd.
+    - simpl in Hhd. injection Hhd as H. now subst.
+  Qed.
+
+  Lemma  canon_trace_add x y y' z f t (Hf : x ~[f]~> y)
+                         (Hy' : y == y')
+                         (Ht : CanonicalTrace t y' z)
+                         (Hfoll : ~can_follow_hd f t) :
+    exists t', exists{z' == z},
+      CanonicalTrace t' x z' /\
+      RestrictedPermutation commute (f :: t) t' /\
+        (hd_error t = hd_error t').
+  Proof.
+    generalize dependent x. generalize dependent y.
+    induction Ht as [|y' v z g t' Hy'v Hfoll' Ht'].
+    - exfalso.
+      unfold not, can_follow_hd in Hfoll.
+      contradiction.
+    - intros y Hyy' x Hxy. simpl in Hfoll.
+      assert (Hfg_canon : canon_rel g f). {
+        clear IHHt'.
+        firstorder.
+      }
+      assert (Hfg_comm : commute f g). {
+        unfold can_follow_hd, can_follow in Hfoll.
+        destruct (commut_dec f g).
+        - assumption.
+        - firstorder.
+      }
+      (* Use commutativity to derive an intermediate state on
+         the [g ∘ f] path: *)
+      assert (exists{v' == v}, x ~[g ∘ f]~> v') as Hv'. {
+        symmetry in Hyy'.
+        morph_shift g y.
+        destruct (Hfg_comm x v') as [Hcomm _].
+        destruct Hcomm as [w Hw].
+        { exists y. firstorder. }
+        exists w. split.
+        - firstorder.
+        - destruct Hw as [_ H1]. now rewrite Hequiv_v_v', H1.
+      }
+      destruct Hv' as [v' [Hxv' Hvv']].
+      specialize (morphism_covariance (mfunCanonTrace t') v v' z Hvv' Ht') as Hw'.
+      destruct Hw' as [w' [Hw' Hww']].
+      (* Case analysis: can we add attach [g] to [t']? *)
+      destruct (can_follow_hd_dec f t').
+      { (* Yes, we can. Proof by construction: *)
+        exists (g :: f :: t'). clear IHHt'.
+        destruct Hxv' as [u [Hg' Hf']].
+        exists w'. repeat split.
+        - constructor 2 with (s' := u).
+          + assumption.
+          + simpl. unfold can_follow. now right.
+          + constructor 2 with (s' := v'); assumption.
+        - now constructor.
+        - assumption.
+      }
+      { (* No, we cannot. Proof by induction: *)
+        destruct Hxv' as [u' [Hxu' Hv'u']].
+        symmetry in Hvv'.
+        specialize (IHHt' H v' Hvv' u' Hv'u').
+        destruct IHHt' as [t'' [z' Ht'']].
+        destruct Ht'' as [[Ht'' [Hpermt'' Hhd]] Hzz'].
+        exists (g :: t''). exists z'. repeat split.
+        - constructor 2 with (s' := u'); auto.
+          eapply can_follow_hd_eq; eauto.
+        - sauto.
+        - assumption.
+      }
+  Qed.
+
+  Theorem canonicalize_trace x z :
+    sufficient_replacement_p _
+      (fun t => x ~[compose_list t]~> z)
+      (fun t => exists{z' == z}, CanonicalTrace t x z').
+  Proof.
+    intros t Ht. generalize dependent z. generalize dependent x.
+    induction t as [|f t].
+    { intros. simpl in Ht. subst.
+      exists []. split.
+      - exists z. sauto.
+      - constructor.
+    }
+    { intros x y Hxy.
+      destruct t as [|g t].
+      - simpl in Hxy. exists [f]. split.
+        + exists y. split.
+          * constructor 2 with (s' := y); [easy | easy | ].
+            constructor.
+          * reflexivity.
+        + repeat constructor.
+      - destruct Hxy as [w [Hxw Hwy]].
+        eapply IHt in Hwy.
+        destruct Hwy as [t' [[y' [Hcanont' Hyy']] Hpermt']].
+        destruct (can_follow_hd_dec f t').
+        + exists (f :: t'). split.
+          * exists y'. split.
+            -- constructor 2 with (s' := w); assumption.
+            -- assumption.
+          * now constructor.
+        + clear IHt.
+          eapply canon_trace_add in Hcanont'; eauto.
+          destruct Hcanont' as [t'' [y'' [Ht'' Hy'']]].
+          destruct Ht'' as [Ht'' [Hperm Hhd]].
+          exists t''. split.
+          * exists y''. split.
+            -- assumption.
+            -- rewrite Hyy', Hy''. reflexivity.
+          * sauto.
+          * reflexivity.
+    }
+  Qed.
+End canonical_trace.
+
+From Coq Require Import ZArith.
+
+Definition PID : Set := list positive.
+
+Section IOHandler.
+  Context {Request : Type} {Reply : Request -> Type}.
+
+  Record IOp := mkIOp {
+      pid : PID;
+      req : Request;
+      ret : Reply req
+    }.
+
+  Class IOHandler := {
+      h_state : Type;
+      h_setoid : Setoid h_state;
+      h_trans : IOp -> @MFun h_state h_state h_setoid h_setoid
+    }.
+End IOHandler.
+
+From Coq Require Import
+  SetoidPermutation.
+
+Section VM.
+  Context `{H : IOHandler}.
+
+  CoInductive Program : Type :=
+  | p_dead : (* Program terminted *)
+      Program
+  | p_cont : (* Program is doing I/O *)
+    forall (pending_req : Request)
+           (continuation : Reply pending_req -> Program),
+      Program
+  | p_spawn : (* Spawn a new process: *)
+    forall (child : Program)
+           (continuation : PID -> Program),
+      Program.
+
+  Record Thread :=
+    { t_pid : PID;
+      t_prog : Program;
+      t_last_child : positive
+    }.
+
+  Record VM :=
+    { threads : list Thread;
+      world : @h_state _ _ H;
+    }.
+
+  Inductive Pick {A : Type} : (list A) -> (A * list A) -> Prop :=
+  | pick_this : forall a l,
+      Pick (a :: l) (a, l)
+  | pick_next : forall a b l l',
+      Pick l (a, l') ->
+      Pick (b :: l) (a, b :: l').
+
+  Definition do_spawn pid lc cont child rest :=
+    let new_pid := pid ++ [lc] in
+    let this_thread := {| t_pid := pid;
+                          t_last_child := Pos.succ lc;
+                          t_prog := cont new_pid
+                       |} in
+    let new_thread := {| t_pid := new_pid;
+                         t_last_child := 1;
+                         t_prog := child
+                      |} in
+    this_thread :: new_thread :: rest.
+
+  Definition do_io pid lc req (ret : Reply req) cont rest :=
+    let new_thread := {| t_pid := pid;
+                         t_last_child := lc;
+                         t_prog := cont ret
+                      |} in
+    new_thread :: rest.
+
+  Inductive VMStep : relation VM :=
+  | vm_proc_down : forall pid lc threads threads' world,
+      Pick threads ({| t_pid := pid; t_last_child := lc; t_prog := p_dead |}, threads') ->
+      VMStep {| threads := threads;
+                world := world
+             |}
+             {| threads := threads';
+                world := world
+             |}
+  | vm_proc_spawn : forall pid lc cont child threads threads' world,
+      Pick threads ({| t_pid := pid; t_last_child := lc; t_prog := p_spawn child cont |}, threads') ->
+      VMStep {| threads := threads;
+                world := world
+             |}
+             {| threads := do_spawn pid lc cont child threads';
+                world := world
+             |}
+  | vm_proc_io : forall pid lc req ret cont threads threads' world world',
+      Pick threads ({| t_pid := pid; t_prog := p_cont req cont; t_last_child := lc |}, threads') ->
+      world ~[h_trans (mkIOp pid req ret)]~> world' ->
+      VMStep {| threads := threads;
+                world := world
+             |}
+             {| threads := do_io pid lc req ret cont threads';
+                world := world'
+             |}.
+
+  Search PermutationA.
+
+  Program Instance vmEquiv : Setoid VM :=
+    {| equiv a b :=
+        PermutationA eq (threads a) (threads b) /\ @equiv _ h_setoid (world a) (world b)
+    |}.
+  Next Obligation.
+  Admitted.
+
+  Program Definition mfunVM : @MFun VM VM vmEquiv vmEquiv :=
+    {| morphism := VMStep;
+    |}.
+  Next Obligation.
+  Admitted.
+
+  (* FIXME *)
+  Fixpoint pid_order (a b : PID) : Prop :=
+    match a, b with
+    | [], [] => True
+    | [], _ => False
+    | _, [] => True
+    | a :: resta, b :: restb =>
+        pid_order resta restb
+    end.
+
+  Global Instance vmStepCanonRel : CanonicalOrder VMStep.
+  Abort.
+
+  Definition initVM (world : h_state) (threads : list Program) : VM :=
+    {|
+      world := world;
+
+      threads :=
+        let go (acc : positive * list Thread) (prog : Program) :=
+          let (pid, threads) := acc in
+          let thread := {| t_pid := [pid]; t_prog := prog; t_last_child := 1 |} in
+          (Pos.succ pid, thread :: threads)
+        in
+        let (_, threads) := fold_left go threads (1%positive, []) in
+        threads;
+    |}.
+End VM.
+
+Global Arguments initVM {_ _} (_ _ _).
+
+Definition ProgramType {Req Ret} (_ : @IOHandler Req Ret) : Type := @Program Req Ret.
+
+Notation "'do' V '<-' I ; C" := (p_cont (I) (fun V => C))
+    (at level 100, C at next level, V name, right associativity) : slot_scope.
+
+Notation "'done'" := (p_dead)
+    (at level 100, right associativity) : slot_scope.
+
+Notation "'call' V '<-' I ; C" := (I (fun V => C))
+    (at level 100, C at next level, V ident,
+     right associativity,
+      only parsing) : slot_scope.
+
+Notation "'spawn' V '<-' I ; C" := (p_spawn (I) (fun V => C))
+    (at level 100, C at next level, V ident,
+      right associativity) : slot_scope.
+
+From LibTx Require Import
+  Storage
+  Instances.List.
+
+Module stor := LibTx.Storage.Classes.
+
+Section storage_handler.
+  Context {Key Val Container : Type} `(Hstor : Storage Key Val Container).
+
+  Inductive StorageReq : Type :=
+  | get : Key -> StorageReq.
+  (* | put : K -> V -> StorageReq *)
+  (* | delete : K -> StorageReq. *)
+
+  Definition StorageRet (req : StorageReq) : Type :=
+    match req with
+    | get k => option Val
+    (* | put k v => True *)
+    (* | delete k => True *)
+    end.
+
+  Program Definition mfunStorageGet (k : Key) (ret : option Val) : @MFun Container Container s_eq_setoid s_eq_setoid :=
+    {|
+      morphism s s' := s = s' /\ ret = stor.get k s;
+    |}.
+  Next Obligation.
+    exists x'. sauto.
+  Qed.
+
+  Instance storageHandler : @IOHandler StorageReq StorageRet :=
+    {|
+      h_state := Container;
+      h_setoid := s_eq_setoid;
+      h_trans :=
+        fun iop =>
+          match iop with
+            {| req := get k; ret := ret |} =>
+              mfunStorageGet k ret
+          end
+    |}.
+End storage_handler.
+
+Global Arguments storageHandler (_ _) {_} (_).
+
+Section test.
+  Let handler := storageHandler nat nat listStorage.
+
+  Let getter (key : nat) : ProgramType handler :=
+        do val <- get key;
+        done.
+
+  Let prog : ProgramType handler :=
+        spawn A <- getter 1;
+        spawn B <- getter 2;
+        done.
+
+  Let initialState := initVM handler [] [prog].
+
+
+  Goal forall t,
+      initialState ~[compose_list t]~> initVM handler [] [] ->
+      t = [].
+  Proof.
+    intros t Ht.
+    unfold initialState, initVM in Ht.
+  Abort.
+End test.
